Source/DafnyStandardLibraries/src/Std/Frames.dfy
@@ -1,12 +1,9 @@
-// RUN: %dafny /compile:0 "%s" > "%t"
-// RUN: %diff "%s.expect" "%t"
-
 module Frames {
 
   // A trait for objects with a Valid() predicate. Necessary in order to
   // generalize some proofs, but also useful for reducing the boilerplate
   // that most such objects need to include.
-  trait {:termination false} Validatable {
+  trait Validatable {
     // Ghost state tracking the common set of objects most
     // methods need to read.
     ghost var Repr: set<object>
